Very close to having AxiomaticSem. ready for send+recv.

Java/src/Logic/AssertionLogic.v
@@ -42,18 +42,6 @@ Definition asn := ILPreFrm Prog_wf_sub asn2.
 Instance ILogicOpsAsn : ILogicOps asn := _.
 Instance ILogicAsn : ILogic asn := _.
 
-Instance BILOperatorsAsn1 : BILOperators asn1 := _.
-Instance BILOperatorsAsn2 : BILOperators asn2 := _.
-Instance BILOperatorsAsn : BILOperators asn := _.
-
-Instance BILogicAsn1 : BILogic asn1 := _.
-Instance BILogicAsn2 : BILogic asn2 := _.
-Instance BILogicAsn  : BILogic asn := _.
-
-Instance IBILogicAsn1 : IBILogic asn1 := _.
-Instance IBILogicAsn2 : IBILogic asn2 := _.
-Instance IBILogicAsn  : IBILogic asn := _.
-
 Local Existing Instance EmbedILPreDropOp.
 Local Existing Instance EmbedILPreDrop.
 Local Existing Instance EmbedOpPropProp.
@@ -61,9 +49,31 @@ Local Existing Instance EmbedPropProp.
 
 Instance EmbedAsnPropOp : EmbedOp Prop asn := _.
 Instance EmbedAsnProp : Embed Prop asn := _.
+ 
+Instance traces_Rel : Rel traces := Equal.
+Instance traces_PreOrder : PreOrder (@rel traces Equal) := _. 
+Definition tasn := ILPreFrm (@rel traces Equal) asn.
 
-Definition sasn := @open var _ asn.
+Instance ILogicOpsTAsn : ILogicOps tasn := _.
+Instance ILogicTAsn : ILogic tasn := _.
 
+Instance BILOperatorsAsn1 : BILOperators asn1 := _.
+Instance BILOperatorsAsn2 : BILOperators asn2 := _.
+Instance BILOperatorsAsn  : BILOperators asn := _.
+Instance BILOperatorsTAsn : BILOperators tasn := _.
+
+Instance BILogicAsn1 : BILogic asn1 := _.
+Instance BILogicAsn2 : BILogic asn2 := _.
+Instance BILogicAsn  : BILogic asn := _.
+Instance BILogicTAsn : BILogic tasn := _.
+
+Instance IBILogicAsn1 : IBILogic asn1 := _.
+Instance IBILogicAsn2 : IBILogic asn2 := _.
+Instance IBILogicAsn  : IBILogic asn := _.
+Instance IBILogicTAsn : IBILogic tasn := _.
+
+Definition sasn := @open var _ tasn.
+ 
 Instance ILOpsSAsn : ILogicOps sasn := _.
 Instance ILogicSAsn : ILogic sasn := _.
 Instance BILOperatorsSAsn : BILOperators sasn := _.
@@ -80,6 +90,9 @@ Local Existing Instance SABIOps.
 Local Existing Instance SABILogic.
 Local Existing Instance pureop_bi_sepalg.
 
+Instance EmbedTAsnPropOp : EmbedOp Prop tasn := _.
+Instance EmbedTAsnProp : Embed Prop tasn := _.
+
 Instance EmbedSasnPureOp : EmbedOp vlogic sasn := _.
 Instance EmbedSasnPure : Embed vlogic sasn := _.
 
@@ -91,6 +104,8 @@ Instance EmbedAsn2SpecOp : EmbedOp spec1 asn2 := _.
 Instance EmbedAsn2Spec   : Embed spec1 asn2 := _.
 Instance EmbedAsnSpecOp  : EmbedOp spec asn := _.
 Instance EmbedAsnSpec    : Embed spec asn := _.
+Instance EmbedTAsnSpecOp : EmbedOp spec tasn := _. 
+Instance EmbedTAsnSpec   : Embed spec tasn := _.
 Instance EmbedSAsnSpecOp : EmbedOp spec sasn := _.
 Instance EmbedSAsnSpec   : Embed spec sasn := _.
 
@@ -115,6 +130,8 @@ Local Instance PureOpAsn2 : @PureOp asn2 := _.
 Local Instance PureAsn2 : Pure PureOpAsn2 := _.
 Local Instance PureOpAsn : @PureOp asn := _.
 Local Instance PureAsn : Pure PureOpAsn := _.
+Local Instance PureOpTAsn : @PureOp tasn := _.
+Local Instance PureTAsn : Pure PureOpTAsn := _.
 Local Instance PureOpSasn : @PureOp sasn := _.
 Local Instance PureSAsn : Pure PureOpSasn := _.
 
@@ -142,6 +159,14 @@ Grab Existential Variables.
   intros h h' Hh H. eapply Hheap; eassumption.
 Defined.
 
+Definition mk_tasn (f: traces -> asn)
+  (Hst: forall P k h tr tr', Equal tr tr' -> f tr P k h -> f tr' P k h) : tasn.
+  refine (mkILPreFrm (fun tr => f tr) _).
+Proof.
+  intros t t' Heq Pr k h H.
+  eapply Hst; eassumption.
+Defined.
+
 Program Definition pointsto_aux (x : ptr) (f : field) (v : val) : asn :=
   mk_asn (fun P k h => subheap ((empty val) [(x, f) <- v]) (get_heap_ptr h)) _ _ _.
 Next Obligation.
@@ -150,7 +175,7 @@ Next Obligation.
   setoid_rewrite H in H0. assumption.
 Qed.
 
-Definition pointsto (p : val) (f : field) (v : val) : asn :=
+Definition pointsto (p : val) (f : field) (v : val) : asn := 
   (p <> null) /\\ pointsto_aux (val_to_ptr p) f v.
 
 Program Definition pointsto_arr_element_aux (x : val) (path : list val) (v : val) : asn :=
