Java/src/Semantics/OperationalSemantics.v
@@ -15,7 +15,7 @@ Section Commands.
   | assign_ok : forall P s h t v
                        (He: eval e s = v),
       assign_sem x e P 1 s h t (Some (stack_add x v s, (h, t))).
-  Program Definition assign_cmd x e := Build_semCmd (assign_sem x e) _ _ _.
+  Program Definition assign_cmd x e := Build_semCmd (assign_sem x e) _ _.
   Next Obligation.
     intros H; inversion H.
   Qed.
@@ -23,11 +23,11 @@ Section Commands.
     unfold frame_property; intros.
     inversion HSem; subst; clear HSem; exists h...
   Qed.
-  Next Obligation.
+  (* Next Obligation.
     unfold increasing_traces; intros.
     inversion HSem; subst.
     reflexivity.
-  Qed.
+  Qed. *)
 
   Inductive read_sem (x y : var) (f : field) : semCmdType :=
   | read_ok : forall ref v P (s : stack) (h : heap) (t : traces)
@@ -38,7 +38,7 @@ Section Commands.
       (Sref   : s y = vptr ref)
       (Snotin : ~ In (ref,f) (get_heap_ptr h)),
       read_sem x y f P 1 s h t None.
-  Program Definition read_cmd x y f := Build_semCmd (read_sem x y f) _ _ _.
+  Program Definition read_cmd x y f := Build_semCmd (read_sem x y f) _ _.
   Next Obligation.
     intros H; inversion H.
   Qed.
@@ -51,11 +51,11 @@ Section Commands.
     destruct (sa_mul_mapstoR HFrame Rmaps) as [[H1 H2] | [H1 H2]]; [assumption|].
     contradiction HSafe; apply read_fail with ref; assumption.
   Qed.
-  Next Obligation.
+  (* Next Obligation.
     unfold increasing_traces; intros.
     inversion HSem; subst.
     reflexivity.
-  Qed.
+  Qed. *)
 
 Require Import Compare_dec.
 
@@ -141,7 +141,7 @@ Require Import Compare_dec.
                   (Smap : List.map (fun e => eval e s) path = vpath)
                   (Sarr : ~ in_heap_arr arr (List.map val_to_nat vpath) (get_heap_arr h)) :
       read_arr_sem x y path P 1 s h t None.
-  Program Definition read_arr_cmd x y path := Build_semCmd (read_arr_sem x y path) _ _ _.
+  Program Definition read_arr_cmd x y path := Build_semCmd (read_arr_sem x y path) _ _.
   Next Obligation.
     intros H. inversion H.
   Qed.
@@ -157,11 +157,11 @@ Require Import Compare_dec.
     eapply read_arr_fail; try eassumption; try reflexivity.
     eapply find_heap_arr_frame; eauto. apply HFrame.
   Qed.
-  Next Obligation.
+  (* Next Obligation.
     unfold increasing_traces; intros.
     inversion HSem; subst.
     reflexivity.
-  Qed.
+  Qed. *)
 
   Inductive write_arr_sem (x : var) (path : list dexpr) (e : dexpr) : semCmdType :=
   | write_arr_ok P arr s h ha' t vpath
@@ -175,7 +175,7 @@ Require Import Compare_dec.
                    (Smap : List.map (fun e' => eval e' s) path = vpath)
                    (Sin  : ~ in_heap_arr arr (List.map val_to_nat vpath) (get_heap_arr h)) :
       write_arr_sem x path e P 1 s h t None.
-  Program Definition write_arr_cmd x path e := Build_semCmd (write_arr_sem x path e) _ _ _.
+  Program Definition write_arr_cmd x path e := Build_semCmd (write_arr_sem x path e) _ _.
   Next Obligation.
     intros H. inversion H.
   Qed.
@@ -197,11 +197,11 @@ Require Import Compare_dec.
     apply H1.
     eapply write_arr_ok; try eassumption; reflexivity.
   Qed.
-  Next Obligation.
+  (* Next Obligation.
     unfold increasing_traces; intros.
     inversion HSem; subst.
     reflexivity.
-  Qed.
+  Qed. *)
 
   Inductive alloc_arr_sem (x : var) (e : dexpr) : semCmdType :=
   | alloc_arr_ok (P : Prog_wf) (s s' : stack) (h : heap) (ha' : heap_arr) (t : traces) (n : nat)
@@ -209,7 +209,7 @@ Require Import Compare_dec.
                  (Sha : alloc_heap_arr n (val_to_nat (eval e s)) (get_heap_arr h) === ha') 
                  (Ss : s' = stack_add x (varr n) s) :
       alloc_arr_sem x e P 1 s h t (Some (s', ((mkheap (get_heap_ptr h) ha'), t))).
-  Program Definition alloc_arr_cmd x e := Build_semCmd (alloc_arr_sem x e) _ _ _.
+  Program Definition alloc_arr_cmd x e := Build_semCmd (alloc_arr_sem x e) _ _.
   Next Obligation.
     intros H; inversion H.
   Qed.
@@ -254,11 +254,11 @@ Require Import Compare_dec.
     specialize (Sfresh_ha i). apply Sfresh_ha.
     destruct (sa_mul_inL HFrame_arr H). assumption.
   Qed.
-  Next Obligation.
+  (* Next Obligation.
     unfold increasing_traces; intros.
     inversion HSem; subst.
     reflexivity.
-  Qed.
+  Qed. *)
     
   Inductive alloc_sem (x : var) (C : class) : semCmdType :=
   | alloc_ok : forall (P : Prog_wf) (s s' : stack) (h : heap) (hp' : heap_ptr) t n fields
@@ -269,7 +269,7 @@ Require Import Compare_dec.
         (SS.fold (fun f h' => add ((n, C), f) (pnull : val) h') fields heap_ptr_unit) hp')
       (Ss0      : s' = stack_add x (vptr (n, C)) s),
       alloc_sem x C P 1 s h t (Some (s', ((mkheap hp' (get_heap_arr h)), t))).
-  Program Definition alloc_cmd x C := Build_semCmd (alloc_sem x C) _ _ _.
+  Program Definition alloc_cmd x C := Build_semCmd (alloc_sem x C) _ _.
   Next Obligation.
     intros H; inversion H.
   Qed.
@@ -291,11 +291,11 @@ Require Import Compare_dec.
     destruct (sa_mul_inR Sh0 H9) as [[H10 H11] | [H10 H11]]; [assumption|].
     apply sa_mulC in H1; destruct (sa_mul_inL H1 H10); intuition.
   Qed.
-  Next Obligation.
+  (* Next Obligation.
     unfold increasing_traces; intros.
     inversion HSem; subst.
     reflexivity.
-  Qed.
+  Qed. *)
 
   Inductive write_sem (x:var) (f:field) (e:dexpr) : semCmdType := 
   | write_ok : forall P (s: stack) (h : heap) (hp' : heap_ptr) t ref v
@@ -308,7 +308,7 @@ Require Import Compare_dec.
       (Sref:   s x = vptr ref)
       (Sin : ~ In (ref, f) (get_heap_ptr h)),
       write_sem x f e P 1 s h t None.
-  Program Definition write_cmd x f e := Build_semCmd (write_sem x f e) _ _ _.
+  Program Definition write_cmd x f e := Build_semCmd (write_sem x f e) _ _.
   Next Obligation.
     intros H; inversion H.
   Qed.
@@ -328,41 +328,35 @@ Require Import Compare_dec.
     eapply write_ok; try eassumption; try reflexivity.
     destruct (sa_mul_inR HFrame_ptr Sin); intuition.
   Qed.
-  Next Obligation.
+  (* Next Obligation.
     unfold increasing_traces; intros.
     inversion HSem; subst.
     reflexivity.
-  Qed.
+  Qed. *)
 
   Inductive send_sem (x v : var) : semCmdType :=
-  | send_ok : forall P (s: stack) (h h': heap) (t t': traces) (tr: trace) (c: stptr)
+  | send_ok : forall P (s: stack) (h mres: heap) (t t': traces) (tr: trace) (c: stptr)
     (Sref: s x = vst c)
-    (Strace: MapsTo c tr t)
-    (Smarshall: marshall (s v) h h')
-    (Sadd: t' = add c (tsend (s v) h' tr) t),
+    (Strace: MapsTo c (tsend (s v) mres tr) t)
+    (Smarshall: marshall (s v) h mres)
+    (Sadd: t' = add c tr t),
     send_sem x v P 1 s h t (Some (s, (h, t')))
-  | send_fail1 : forall P (s: stack) (h: heap) (t: traces) (c: stptr)
-    (Sref: s x = vst c)
-    (Strace: ~ In c t),
-    (* There is no known trace for this channel *)
-    send_sem x v P 1 s h t None
-  | send_fail2 : forall P (s: stack) (h h': heap) (t: traces) (tr: trace) (c: stptr)
+  | send_fail2 : forall P (s: stack) (h mres: heap) (t: traces) (tr: trace) (c: stptr)
   	(Sref: s x = vst c)
-    (Strace: MapsTo c tr t)
-    (Smarshalls: ~ marshall (s v) h h'),
+    (Strace: MapsTo c (tsend (s v) mres tr) t)
+    (Smarshalls: ~ marshall (s v) h mres),
     (* Unable to marshall the value pointed to by (s v) in the heap h *)
     send_sem x v P 1 s h t None
   .  
-  Program Definition send_cmd x v := Build_semCmd (send_sem x v) _ _ _.
+  Program Definition send_cmd x v := Build_semCmd (send_sem x v) _ _.
   Next Obligation.
     intros H; inversion H.
   Qed.
   Next Obligation.
     unfold frame_property; intros.
     inversion HSem. subst; clear HSem.
-    exists h. split.
-    assumption.
-    assert (DisjointHeaps frame h' \/ ~DisjointHeaps frame h') by admit.
+    exists h; split; [assumption |]. 
+    assert (DisjointHeaps frame mres \/ ~DisjointHeaps frame mres) by admit (* fangel *).
     destruct H.
     * eapply send_ok; [ apply Sref | apply Strace | | reflexivity].
       eapply marshall_into_smaller in H; [| apply HFrame | apply Smarshall].
@@ -375,23 +369,22 @@ Require Import Compare_dec.
       + eapply send_ok; [apply Sref | apply Strace | | reflexivity].
         eapply marshall_into_unit; [ apply H | apply Smarshall].
   Qed.
-  Next Obligation.
+  (* Next Obligation.
     unfold increasing_traces; intros.
     inversion HSem; subst.
     eapply traces_lte_existing; [apply Strace |].
     repeat constructor.
-  Qed.
+  Qed. *)
 
   Inductive recv_sem (v x : var) : semCmdType :=
-  | recv_ok : forall P (s: stack) (h ih rh h': heap) (t t': traces) (tr: trace) (c: stptr) (rv : sval)
+  | recv_ok : forall P (s: stack) (h rh h': heap) (t t': traces) (tr: trace) (c: stptr) (rv : sval)
     (Sref: s x = vst c)
-    (Strace: MapsTo c tr t)
-    (Smarshall: marshall rv ih rh)
+    (Strace: MapsTo c (trecv rv rh tr) t)
     (Snewheap : sa_mul h rh h')
-    (Sadd: t' = add c (trecv rv rh tr) t),
+    (Sadd: t' = add c tr t),
     recv_sem v x P 1 s h t (Some (stack_add v rv s, (h', t')))
   .
-  Program Definition recv_cmd v x := Build_semCmd (recv_sem v x) _ _ _.
+  Program Definition recv_cmd v x := Build_semCmd (recv_sem v x) _ _.
   Next Obligation.
     intros H; inversion H.
   Qed.
@@ -414,7 +407,7 @@ Require Import Compare_dec.
         }
         rewrite <- Heqh' in H.
         exfalso. apply Hneq. apply H.
-     * eapply recv_ok; [apply Sref | apply Strace | apply Smarshall | | reflexivity].
+     * eapply recv_ok; [apply Sref | apply Strace | | reflexivity].
        rewrite Heqh'. apply DisjointHeaps_sa_mul.
        apply sa_mulC in HFrame.
        eapply sa_mulA in Snewheap; [| apply HFrame].
@@ -422,12 +415,12 @@ Require Import Compare_dec.
        apply sa_mul_DisjointHeaps in H0.
        apply H0.
   Qed.
-  Next Obligation.
+  (* Next Obligation.
     unfold increasing_traces; intros.
     inversion HSem; subst.
     eapply traces_lte_existing; [ apply Strace |].
     repeat constructor.
-  Qed.
+  Qed. *)
 
   Fixpoint create_stack (ps : list var) (vs : list val) : stack :=
     match ps, vs with
@@ -457,7 +450,7 @@ Require Import Compare_dec.
       (HSem    : sc P n (create_stack ps (eval_exprs s es)) h t (Some (sr, (hr, tr)))),
       call_sem rvar C m es c sc P (S n) s h t
         (Some (stack_add rvar (eval rexpr sr) s, (hr, tr))).
-  Program Definition call_cmd rvar C m es c sc := Build_semCmd (call_sem rvar C m es c sc) _ _ _.
+  Program Definition call_cmd rvar C m es c sc := Build_semCmd (call_sem rvar C m es c sc) _ _.
   Next Obligation.
     intros H; inversion H.
   Qed.
@@ -467,12 +460,12 @@ Require Import Compare_dec.
     edestruct (@cmd_frame sc) as [h1 [HFrame1 HSem1]]...
     intros k HLe HFail; apply HSafe with (S k); [omega |]...
   Qed.
-  Next Obligation with eauto using call_sem.
+  (* Next Obligation with eauto using call_sem.
     unfold increasing_traces; intros.
     inversion HSem; subst.
     apply semCmd_traces_lte in HSem0; [apply HSem0 |].
     intros k HLe HFail; apply HSafe with (S k); [omega |]...
-  Qed.
+  Qed. *)
 
   Inductive semantics : cmd -> semCmd -> Prop :=
   | semassign : forall x e,
@@ -595,42 +588,47 @@ End Commands.
   Local Transparent ILPre_Ops.
   Local Transparent ILFun_Ops.
 
-  Definition triple (P Q : sasn) (c : cmd) :=
+  Definition triple (P Q : sasn) (* st st': open STs *) (c : cmd) :=
     Forall sc : semCmd, (semantics c sc) ->> {{P}} sc {{Q}}.
 
+ (* Notation " '{[' P '|' st ']}' c '{[' Q '|' st' ']}' " := (triple P Q st st' c) (at level 89,
+    format " {[ P | st ]} '/' c '/' {[ Q | st' ]} "). *)
   Notation " '{[' P ']}' c '{[' Q ']}' " := (triple P Q c) (at level 89,
     format " {[ P ]} '/' c '/' {[ Q ]} ").
+    
 
   Add Parametric Morphism : triple with signature
-    lentails --> lentails ++> eq ==> lentails
+    lentails --> lentails ++> eq (*++> eq ++> eq*) ==> lentails
     as triple_entails_m.
   Proof.
-    intros p p' Hp q q' Hq c.
+    intros p p' Hp q q' Hq (* st st' *) c.
     unfold triple. 
     setoid_rewrite Hq; setoid_rewrite <- Hp. reflexivity.
   Qed.
 
 Open Scope open_scope.
 
-  Definition method_spec C m (ps : list var) (rn : var) (P Q : sasn) := (
+  Definition method_spec C m (ps : list var) (rn : var) (P Q : sasn) (* st st': open STs *) := (
     NoDup (rn :: ps) /\\
     Exists ps' : (list var), Exists c : cmd, Exists re : dexpr,
       [prog] (fun X : Prog_wf => method_lookup X C m (Build_Method ps' c re)
         /\ length ps = length ps' /\
         (forall x, List.In x ps' -> ~ SS.In x (modifies c)))
       //\\ {[ P //! zip ps (List.map var_expr ps') ]}
-         c {[ Q //! zip (rn :: ps) (eval re :: (List.map var_expr ps'))]}
+         c {[ Q //! zip (rn :: ps) (eval re :: (List.map var_expr ps')) ]}
     ).
 
+  (*Notation " C ':.:' m |-> ps {{ P | st }}-{{ r , Q | st' }} " :=
+    (method_spec C m ps r P Q st st') (at level 60).*)
   Notation " C ':.:' m |-> ps {{ P }}-{{ r , Q }} " :=
     (method_spec C m ps r P Q) (at level 60).
 
   Add Parametric Morphism : method_spec with signature
     eq ==> eq ==> eq ==> eq ==>
-      lentails --> lentails ++> lentails
+      lentails --> lentails ++> (* eq ++> eq ++>*)  lentails
     as method_spec_entails_m.
   Proof.
-    intros C m ps rn P P' HP Q Q' HQ. unfold method_spec.
+    intros C m ps rn P P' HP Q Q' HQ (* st st' *). unfold method_spec.
     (* Unravel the two almost identical sides of the entailment first because
         setoid_rewrite doesn't seem to go under these binders. *)
     apply lpropandL; intro H. apply lpropandR; [assumption|].
@@ -642,14 +640,14 @@ Open Scope open_scope.
 
   Add Parametric Morphism : method_spec with signature
     eq ==> eq ==> eq ==> eq ==>
-      lequiv ==> lequiv ==> lequiv
+      lequiv ==> lequiv ==> (* eq ==> eq ==> *) lequiv
     as method_spec_bientails_m.
   Proof.
     split; apply method_spec_entails_m; try rewrite ?H, ?H0; reflexivity.
   Qed.
 
 
-  Lemma c_triple_zero P (p q : sasn) (c : cmd) :
+  Lemma c_triple_zero P (p q : sasn) (* st st': open STs *) (c : cmd) :
     ({[ p ]} c {[ q ]}) P 0.
   Proof.
     intros sc n Hn Q HPQ sem R k m s h t HQR Hk Hv Hp.
@@ -680,13 +678,13 @@ Open Scope open_scope.
 
 Section StructuralRules.
 
-  Lemma triple_false (G : spec) (Q : sasn) c :
+  Lemma triple_false (G : spec) (Q : sasn) (* st st': open STs *) c :
     G |-- {[lfalse]} c {[Q]}.
   Proof.
     intros n; simpl in *; intros; destruct H4.
   Qed.
 
-  Lemma roc (P P' Q Q' : sasn) c (G : spec)
+  Lemma roc (P P' Q Q' : sasn) (* st st': open STs *) c (G : spec)
     (HPre  : P  |-- P')
     (HPost : Q' |-- Q)
     (Hc    : G  |-- {[P']} c {[Q']}) :
@@ -697,7 +695,7 @@ Section StructuralRules.
     lforallL sc. apply lpropimplL; [assumption|]. apply rule_of_consequence; assumption.
   Qed.
 
-  Lemma roc_pre (P P' Q : sasn) c G
+  Lemma roc_pre (P P' Q : sasn) (* st st': open STs *) c G
     (HPre : P |-- P')
     (Hc   : G |-- {[P']} c {[Q]}) :
     G |-- {[P]} c {[Q]}.
@@ -705,7 +703,7 @@ Section StructuralRules.
   	eapply roc; eassumption || reflexivity.
   Qed.
 
-  Lemma roc_post (P Q Q' : sasn) c G
+  Lemma roc_post (P Q Q' : sasn) (* st st': open STs *) c G
     (Hc : G  |-- {[P]} c {[Q']})
     (HPost : Q' |-- Q) :
     G |-- {[P]} c {[Q]}.
@@ -742,7 +740,7 @@ Section StructuralRules.
   Qed.
   Implicit Arguments rule_frame [[P] [Q] [R] [c] [G]].
 
-  Lemma exists_into_precond2 {A} (P: A -> sasn) c q :
+  Lemma exists_into_precond2 {A} (P: A -> sasn) (* st st': open STs *) c q :
     (Forall x, {[P x]} c {[q]}) -|- {[Exists x, P x]} c {[q]}.
   Proof.
     unfold triple; setoid_rewrite <- exists_into_precond; split.
@@ -752,7 +750,7 @@ Section StructuralRules.
       lforallL sc. apply lpropimplL; [assumption | lforallL x; reflexivity].
   Qed.
   
-  Lemma existentialise_triple (x : var) (P Q : sasn) c (G : spec) 
+  Lemma existentialise_triple (x : var) (P Q : sasn) (* st st': open STs *) c (G : spec) 
 	(H : forall (v : val), G |-- {[@lembedand vlogic sasn _ _ (open_eq (x/V) (`v)) P]} c {[Q]}) :
     G |-- {[P]} c {[Q]}.
   Proof.
