Java/src/Semantics/SemCmd.v
@@ -19,17 +19,17 @@ Section Commands.
       (HSafe  : forall m, m <= n -> safe c P m s h t)
       (HSem   : c P n s big t (Some (s', (big', t')))),
       exists h', sa_mul h' frame big' /\ c P n s h t (Some (s', (h', t'))).
-  Definition increasing_traces (c : semCmdType) :=
+  (* Definition increasing_traces (c : semCmdType) :=
     forall P s s' h h' n t t'
       (HSafe  : forall m, m <= n -> safe c P m s h t)
       (HSem : c P n s h t (Some (s', (h', t')))),
-      traces_lte t t'.
+      traces_lte t t'. *)
 
   Record semCmd := {
     cmd_rel   :> Prog_wf -> nat -> stack -> heap -> traces -> option (stack * (heap * traces)) -> Prop;
     cmd_zero  :  forall P s h t cfg, ~(cmd_rel P 0 s h t cfg);
-    cmd_frame :  frame_property cmd_rel;
-    cmd_trace :  increasing_traces cmd_rel
+    cmd_frame :  frame_property cmd_rel (*;
+    cmd_trace :  increasing_traces cmd_rel *)
   }.
 
   Definition not_modifies (c : semCmdType) x : Prop :=
@@ -41,7 +41,7 @@ Section Commands.
     intros; apply cmd_zero.
   Qed.
   
-  
+  (*
   Lemma semCmd_traces_lte : forall (c : semCmd) P s s' h h' t t' n
     (HSafe  : forall m, m <= n -> safe c P m s h t) 
     (HSem: c P n s h t (Some (s', (h', t')))),
@@ -53,6 +53,7 @@ Section Commands.
     exists x.
     apply H.
   Qed.
+  *)
 
   Global Opaque sa_mul.
 
@@ -61,24 +62,24 @@ Section Commands.
   Program Definition later_cmd (c : semCmd) : semCmd := Build_semCmd
     (fun P n => match n return stack -> heap -> traces -> option (stack * (heap * traces)) -> Prop with
                   | O => fun _ _ _ _ => False
-                  | S n => c P n end) _ _ _.
+                  | S n => c P n end) _ _.
   Next Obligation.
     unfold frame_property; intros.
     destruct n as [| n]; unfold safe in HSafe; simpl in *; [contradiction |].
     eapply cmd_frame; eauto. 
     intros m HLe HFail; apply (HSafe (S m)); auto with arith.
   Qed.
-  Next Obligation.
+  (* Next Obligation.
     unfold increasing_traces; intros.
     destruct n as [| n]; unfold safe in HSafe; simpl in *; [contradiction |].
     eapply cmd_trace; eauto.
     intros m HLe HFail; apply (HSafe (S m)); auto with arith.
-  Qed.
+  Qed. *)
   (* Skip *)
 
   Inductive skip_sem : semCmdType :=
   | s_ok : forall P s h t, skip_sem P 1 s h t (Some (s, (h, t))).
-  Program Definition skip_cmd := @Build_semCmd skip_sem _ _ _.
+  Program Definition skip_cmd := @Build_semCmd skip_sem _ _.
   Next Obligation.
     intros H. inversion H.
   Qed.
@@ -87,11 +88,11 @@ Section Commands.
     inversion HSem; subst; clear HSem.
     exists h; auto using skip_sem.
   Qed.
-  Next Obligation.
+  (*Next Obligation.
     unfold increasing_traces; intros.
     inversion HSem; subst; clear HSem.
     reflexivity.
-  Qed.
+  Qed.*)
 
   (* Seq *)
   Inductive seq_sem (c1 c2 : semCmd) : semCmdType :=
@@ -106,7 +107,7 @@ Section Commands.
       c1 P n  s  h  t  (Some (s0, (h0, t0))) ->
       c2 P n0 s0 h0 t0 (Some (s1, (h1, t1))) ->
       seq_sem c1 c2 P (S (n + n0)) s h t (Some (s1, (h1, t1))).
-  Program Definition seq_cmd c1 c2 := @Build_semCmd (seq_sem c1 c2) _ _ _.
+  Program Definition seq_cmd c1 c2 := @Build_semCmd (seq_sem c1 c2) _ _.
   Next Obligation.
     intros H; inversion H.
   Qed.
@@ -118,7 +119,7 @@ Section Commands.
     + edestruct (@cmd_frame c2) with(n:=n1) as [hr [HFrame1 HSem1]]...
       intros m HLe HFail; apply HSafe with (S (n0 + m)); [omega | ]...
   Qed.
-  Next Obligation with eauto using seq_sem.
+  (* Next Obligation with eauto using seq_sem.
     unfold increasing_traces; intros.
     inversion HSem; subst; clear HSem.
     assert (traces_lte t t1). {
@@ -130,7 +131,7 @@ Section Commands.
       intros m HLe HFail; apply HSafe with (S (n0 + m)); [omega | ]...
 	}
     transitivity t1; assumption.
-  Qed.    
+  Qed. *)   
 
   (* Nondet *)
   Inductive nondet_sem (c1 c2 : semCmd) : semCmdType :=
@@ -146,7 +147,7 @@ Section Commands.
   | nondet_okR   : forall P n s s' h h' t t',
       c2 P n s h t (Some (s', (h', t'))) ->
       nondet_sem c1 c2 P (S n) s h t (Some (s', (h', t'))).
-  Program Definition nondet_cmd c1 c2 := @Build_semCmd (nondet_sem c1 c2) _ _ _.
+  Program Definition nondet_cmd c1 c2 := @Build_semCmd (nondet_sem c1 c2) _ _.
   Next Obligation.
     intros H; inversion H.
   Qed.
@@ -158,14 +159,14 @@ Section Commands.
     + edestruct (@cmd_frame c2) as [h0 [HFrame0 HSem0]]...
       intros m HLe HFail; apply HSafe with (S m); [omega |]...
   Qed.
-  Next Obligation with eauto using nondet_sem.
+  (* Next Obligation with eauto using nondet_sem.
     unfold increasing_traces; intros.
     inversion HSem; subst; clear HSem.
     + apply semCmd_traces_lte in H5; [ apply H5 |].
       intros m HLe HFail; apply HSafe with (S m); [omega |]...
     + apply semCmd_traces_lte in H5; [ apply H5 |].
       intros m HLe HFail; apply HSafe with (S m); [omega |]...
-  Qed.    
+  Qed. *)   
 
   (* Kleene star *)
   Inductive kleene_sem (c : semCmd) : semCmdType :=
@@ -182,7 +183,7 @@ Section Commands.
       c P n s h t (Some (s0, (h0, t0))) ->
       kleene_sem c P n0 s0 h0 t0 (Some (s1, (h1, t1))) ->
       kleene_sem c P (S (n + n0)) s h t (Some (s1, (h1, t1))).
-  Program Definition kleene_cmd c := @Build_semCmd (kleene_sem c) _ _ _.
+  Program Definition kleene_cmd c := @Build_semCmd (kleene_sem c) _ _.
   Next Obligation.
     intros H; inversion H.
   Qed.
@@ -195,7 +196,7 @@ Section Commands.
     + destruct (IHHSem (eq_refl _) h' HFrame0) as [hr [HFrame1 HSem1]]...
       intros m HLe HFail; apply HSafe with (S (n + m)); [omega |]...
   Qed.
-  Next Obligation with eauto using kleene_sem.
+  (* Next Obligation with eauto using kleene_sem.
     unfold increasing_traces; intros.
     remember (Some (s', (h', t'))) as cfg; induction HSem;
     inversion Heqcfg; subst; intros; clear Heqcfg...
@@ -207,7 +208,7 @@ Section Commands.
     transitivity t0; [apply H0 |].
     apply IHHSem; [| reflexivity].
     intros m HLe HFail; apply HSafe with (S (n + m)); [omega |]...
-  Qed.
+  Qed. *)
 
   (* TODO: update the description
      assume command -- this command is a bit of a hack that just skips if
@@ -215,7 +216,7 @@ Section Commands.
      using nondeterministic choice/Kleene star *)
   Inductive assume_sem (p : vlogic) : semCmdType :=
   | assume_ok : forall P s h t, p s -> assume_sem p P 1 s h t (Some (s, (h, t))).
-  Program Definition assume_cmd P := @Build_semCmd (assume_sem P) _ _ _.
+  Program Definition assume_cmd P := @Build_semCmd (assume_sem P) _ _.
   Next Obligation.
     intros H; inversion H.
   Qed.
@@ -224,11 +225,11 @@ Section Commands.
     remember (Some (s', (big', t'))) as cfg; induction HSem.
     inversion Heqcfg; subst; eauto using assume_sem.
   Qed.
-  Next Obligation.
+  (* Next Obligation.
     unfold increasing_traces; intros.
     inversion HSem; subst. 
     reflexivity.
-  Qed.
+  Qed. *)
 
   Lemma assume_inv P e n s s0 h h0 t t0 (HSem : assume_cmd e P n s h t (Some (s0, (h0, t0)))) : 
       s = s0 /\ h = h0 /\ t = t0.
@@ -242,7 +243,7 @@ Section Commands.
     assert_sem p P 1 s h t (Some (s, (h, t)))
   | assert_fail : forall P s h t (HNP : ~p s),
     assert_sem p P 1 s h t None.
-  Program Definition assert_cmd p := @Build_semCmd (assert_sem p) _ _ _.
+  Program Definition assert_cmd p := @Build_semCmd (assert_sem p) _ _.
   Next Obligation.
     intros H; inversion H.
   Qed.
@@ -250,19 +251,40 @@ Section Commands.
     unfold frame_property; simpl; intros.
     inversion HSem; subst; eauto using assert_sem.
   Qed.
-  Next Obligation.
+  (* Next Obligation.
     unfold increasing_traces; intros.
     inversion HSem; subst.
     reflexivity.
-  Qed.
+  Qed. *)
 
-  (* |= {p}c{q} *)
+  (* |= {p}c{q} )
+  Program Definition sem_triple (p q : sasn) (st st': open STs) (c : semCmd) : spec :=
+    mk_spec (fun P n => forall P' m k s h t, Prog_wf_sub P P' -> m <= n -> k <= m -> 
+                                           p s P' m h ->
+      (STs_traces P' (st s) t -> safe c P' k s h t) /\
+      (forall t' h' s',  
+      	c P' k s h t (Some (s', (h', t'))) ->
+      		((q s' P' (m - k) h')
+      		/\
+            (STs_traces P' (st' s') t' -> STs_traces P' (st s) t))
+      )
+    ) _ _.
+  Next Obligation.
+    apply H0; try eassumption.
+    etransitivity; eassumption.
+  Qed.
+  *)
   
   Program Definition sem_triple (p q : sasn) (c : semCmd) : spec :=
     mk_spec (fun P n => forall P' m k s h t, Prog_wf_sub P P' -> m <= n -> k <= m -> 
-                                           p s P' m h ->
-      safe c P' k s h t /\
-      forall t' h' s', c P' k s h t (Some (s', (h', t'))) -> (q s' P' (m - k) h')) _ _.
+                                           p s t P' m h ->
+      (safe c P' k s h t) /\
+      (forall t' h' s',  
+      	c P' k s h t (Some (s', (h', t'))) ->
+      		(q s' t' P' (m - k) h')
+      		
+      )
+    ) _ _.
   Next Obligation.
     apply H0; try eassumption.
     etransitivity; eassumption.
@@ -274,6 +296,30 @@ End Commands.
   Local Transparent ILPre_Ops.
   Local Transparent ILFun_Ops.
 
+  (*
+  Add Parametric Morphism : sem_triple with signature
+    lentails --> lentails ++> eq ++> eq ++> eq ==> lentails
+    as sem_triple_entails_m.
+  Proof.
+    intros p p' Hp q q' Hq st st' c n x H P m k s h t HP Hmn Hkm Hp'.
+    apply Hp in Hp'; try apply _.    
+    simpl in *.
+    specialize (H _ _ _ _ _ t HP Hmn Hkm Hp').
+    destruct H as [Hsafe H].
+    split; [assumption|].
+    intros t' h' s'; split.
+    * apply Hq.
+      specialize (H _ _ _ H0).
+      apply H.
+    * specialize (H _ _ _ H0).
+      apply H.
+  Qed.
+
+  Add Parametric Morphism : sem_triple with signature
+    lequiv ==> lequiv ==> eq ==> eq ==> eq ==> lequiv
+    as sem_triple_lequiv_m.
+  *)
+  
   Add Parametric Morphism : sem_triple with signature
     lentails --> lentails ++> eq ==> lentails
     as sem_triple_entails_m.
@@ -284,9 +330,11 @@ End Commands.
     specialize (H _ _ _ _ _ t HP Hmn Hkm Hp').
     destruct H as [Hsafe H].
     split; [assumption|].
-    intros t' h' s' Hc.
+    
+    intros t' h' s' HC.
     apply Hq.
-    apply H in Hc. assumption.
+    specialize (H _ _ _ HC).
+    apply H.
   Qed.
 
   Add Parametric Morphism : sem_triple with signature
@@ -301,5 +349,8 @@ End Commands.
 
 Implicit Arguments Build_semCmd [].
 
+(*
+Notation "{{ p | st }} c {{ q | st' }}" := (sem_triple p q st st' c) (at level 89,
+  format "{{ p | st }} '/ '  c '/ '  {{ q | st' }}"). *)
 Notation "{{ p }} c {{ q }}" := (sem_triple p q c) (at level 89,
   format "{{ p }} '/ '  c '/ '  {{ q }}").
