Java/src/Logic/ST.v
@@ -1,0 +1,116 @@
+Require Import ILogic ILInsts SepAlg BILogic BILInsts IBILogic SepAlgMap Maps String Rel.
+Require Import RelationClasses Setoid Morphisms Program. 
+Require Import MapInterface MapFacts.
+Require Import Open Stack Subst Lang OpenILogic Pure ILEmbed PureInsts.
+Require Import UUSepAlg SepAlgInsts.
+Require Import Heap AssertionLogic Traces SemCmd SemCmdRules.
+
+Inductive ST : Type :=
+  | st_end : ST
+  | st_send : var -> sasn -> ST -> ST
+  | st_recv : var -> sasn -> ST -> ST 
+  .
+
+Definition STs := Map [stptr, ST].
+
+Definition singleton_STs (x : var) (st: open ST) : open STs := fun s => add (val_to_stptr (s x)) (st s) (empty _).
+
+Fixpoint subst_ST (x : var) (v : val) (t : ST) : ST :=
+  match t with
+  | st_end => st_end
+  | st_send x' A t' => st_send x' (apply_subst A (subst1 `v x)) (subst_ST x v t')
+  | st_recv x' A t' => st_recv x' (apply_subst A (subst1 `v x)) (subst_ST x v t')
+  end.
+
+Definition prune_STs (x : var) (st: open STs) : open STs := fun s => 
+	match (s x) with
+	  | vst c => remove c (st s)
+	  | _ => st s
+	end.
+
+Definition subst_STs (x : var) (v : val) (t : STs) : STs := map (subst_ST x v) t.
+
+Inductive ST_trace : Prog_wf -> traces -> ST -> trace -> Prop :=
+  | stt_init : forall (p : Prog_wf) (trs : traces), ST_trace p trs st_end tinit
+  | stt_send : forall (p : Prog_wf) (trs : traces) (t : ST) (v : val) (h : heap) (tr : trace)
+  			   (HGuard: forall (x : var) (A : sasn) (t' : ST),
+  			     t = (st_send x A t') ->
+  			     (apply_subst A (subst1 `v  x)) (stack_empty var) trs p O h -> 
+  			     ST_trace p trs (subst_ST x v t') tr
+  			   ),
+               ST_trace p trs t (tsend v h tr)
+  | stt_recv : forall (p : Prog_wf) (trs : traces) (t : ST) (v : val) (h : heap) (tr : trace)
+  			   (HGuard: forall (x : var) (A : sasn) (t' : ST),
+  			     t = (st_recv x A t') ->
+  			     (apply_subst A (subst1 `v  x)) (stack_empty var) trs p O h /\ 
+  			     ST_trace p trs (subst_ST x v t') tr
+  			   ),
+               ST_trace p trs t (trecv v h tr)
+  .
+
+Local Transparent ILPre_Ops.
+Local Transparent ILFun_Ops.
+Local Transparent BILPre_Ops.
+Local Transparent BILFun_Ops.
+
+Instance ST_trace_m : Proper (eq ==> Equal ==> eq ==> eq ==> iff) ST_trace.
+Proof.
+  intros P P' HPP' trs trs' HtrsEqual tr tr' Htreq t t' Hteq.
+  split; intro Hstt; subst.
+  - induction Hstt.
+    * apply stt_init.
+    * apply stt_send.
+      intros.
+      apply H with (A := A); [ apply H0 | | apply HtrsEqual ].
+      solve_model H1; [| congruence].
+      symmetry; apply HtrsEqual.
+    * apply stt_recv.
+      intros.
+      specialize (HGuard _ _ _ H).
+      destruct HGuard as [HP Hstt].
+      split.
+      + solve_model HP; congruence.
+      + admit (* fangel *).
+  - induction Hstt.
+    * apply stt_init.
+    * apply stt_send.
+      intros.
+      apply H with (A := A); [ apply H0 | | apply HtrsEqual ].
+      solve_model H1; congruence.
+    * apply stt_recv.
+      intros.
+      specialize (HGuard _ _ _ H).
+      destruct HGuard as [HP Hstt].
+      split.
+      + solve_model HP; congruence.
+      + admit (* fangel *).
+Qed.
+
+Definition STs_traces (P : Prog_wf) (t : STs) (tr : traces) : Prop := forall k t', MapsTo k t' t -> exists tr', MapsTo k tr' tr /\ ST_trace P (remove k tr) t' tr'.
+
+
+Program Definition has_ST (c : val) (t : ST) : tasn := 
+  mk_tasn (fun trs => mk_asn (fun P k h => forall P' tr, Prog_wf_sub P P' -> MapsTo (val_to_stptr c) tr trs -> ST_trace P' (remove (val_to_stptr c) trs) t tr) _ _ _) _.
+Next Obligation.
+  assert (Prog_wf_sub P P'0).
+    transitivity P'; assumption.
+  apply H0; assumption.
+Defined.
+Next Obligation.
+  rewrite <- H in H2.
+  rewrite <- H.
+  apply H0; assumption.
+Defined.
+
+Module STNotations.
+ 
+	(* Notation " x ':' t " := (singleton_STs x t) (at level 88, left associativity) : st_scope. *)
+ 
+	Notation " x ':' t " := (has_ST x t) (at level 88, left associativity) : st_scope.
+
+	Notation " '!' x ',{' P '}.' t " := (st_send x P t) (at level 88, left associativity) : st_scope.
+	Notation " '&' x ',{' P '}.' t " := (st_recv x P t) (at level 88, left associativity) : st_scope.
+
+	Open Scope st_scope.
+
+End STNotations.
