Java/src/Semantics/SemCmdRules.v
@@ -51,8 +51,9 @@ Section Rules.
       intros n Pr Hc Pr' m k s h t HPr Hmn Hkm HP; simpl.
       destruct (Hc _ _ _ s h t HPr Hmn Hkm) as [HSafe HQ].
       + apply HPre; apply HP.
-      + split; [apply HSafe|intros t' h' s' H]. 
-        apply HPost. apply HQ in H. apply H.
+      + split; [apply HSafe|intros t' h' s' H]. (* split. *)
+        - apply HPost. specialize (HQ _ _ _ H). apply HQ.
+        (* - specialize (HQ _ _ _ H). apply HQ. *)
     Qed.
 
     Definition not_modifies (c : semCmd) (x : var) : Prop :=
@@ -65,29 +66,37 @@ Section Rules.
       {{ P ** R }} c {{ Q ** Exists vs, apply_subst R (subst_fresh vs xs) }}.
     Proof.
       intros.
-      intros ? PP HSpec PP' ? ? ? ? ? HPP' Hmn Hkm [h1 [h2 [HSub [HP HR]]]]; split.
+      intros PP n HSpec PP' ? ? ? ? ? HPP' Hmn Hkm [h1 [h2 [HSub [HP HR]]]]; split.
       (* safety *)
-      { destruct (HSpec _ m k s h t0 HPP' Hmn Hkm) as [HS _]; [ | assumption].
+      { destruct (HSpec _ m k s h t HPP' Hmn Hkm) as [HS _]; [ | assumption].
         solve_model HP. exists h2; apply HSub.
       }
       (* correctness *)
       intros ? ? ? HSem. 
-      destruct (@cmd_frame c PP' s s' h h' h2 h1 k t0 t') as [h'' [HBig Hc]]. 
+      destruct (@cmd_frame c PP' s s' h h' h2 h1 k t t') as [h'' [HBig Hc]]. 
       + assumption.
-      + intros l Hle. destruct (HSpec _ m l s h1 t0 HPP' Hmn) as [HS _];
-        assumption || omega.
+      + intros l Hle.
+        destruct (HSpec _ m l s h1 t HPP' Hmn) as [HS _]; [ omega | assumption |].
+        apply HS.
       + assumption.
-      + destruct (HSpec _ m k s h1 t0 HPP' Hmn Hkm) as [_ HC]. 
+      + destruct (HSpec _ m k s h1 t HPP' Hmn Hkm) as [_ HC]. 
         * apply HP.
         * specialize (HC t' h'' s' Hc).
-          exists h'', h2, HBig. split. assumption.
+          (* destruct HC as [HC Hst].
+          split; [| assumption]. *)
+          exists h'', h2, HBig. split; [assumption |].
           simpl. exists s. unfold apply_subst.
           solve_model HR.
-          apply functional_extensionality. intros x.
-          unfold stack_subst, subst_fresh.
-          destruct (in_dec Rel.dec_eq x xs) as [|HNotIn]; [reflexivity|].
-          simpl. unfold not_modifies in HMod. eapply HMod; eassumption.
-  Qed.
+          - unfold Rel.rel, MapInterface.Equal.
+            intros x.
+            admit (* fangel, tasn *).
+          - apply functional_extensionality. intros x.
+            unfold stack_subst, subst_fresh.
+            destruct (in_dec Rel.dec_eq x xs) as [|HNotIn]; [reflexivity|].
+            unfold not_modifies in HMod. 
+            specialize (HMod _ HNotIn _ _ _ _ _ _ _ _ HSem).
+            apply HMod.
+    Qed.
 
     Lemma conj_rule G P1 P2 Q1 Q2 c 
       (H1 : G |-- {{P1}} c {{Q1}})
@@ -97,7 +106,12 @@ Section Rules.
       intros n P HPP HG.
       simpl. intros m k s h t HPP' Hm Hk [HP1 HP2]. split.
       + eapply H1; eauto.
-      + split; [eapply H1|eapply H2]; eauto.
+      + intros t' h' s' Hsem.
+        (* split *)
+        - split; [eapply H1|eapply H2]; eauto.
+        (* - edestruct H1; try eassumption.
+          specialize (H0 t' h' s' Hsem).
+          apply H0. *)
     Qed.
 
   End StructuralRules.
@@ -107,64 +121,79 @@ Section Rules.
     Lemma skip_rule P : |-- {{P}}skip_cmd {{P}}.
     Proof.
       intros n Pr HPP Pr' m k s h t _ Hmn Hkm HP; split.
-      + intro H; inversion H.
+      + intros H; inversion H.
       + intros t' h' s' HSem; inversion HSem; subst.
+        (* split; [|intros; assumption]. *)
         solve_model HP.
     Qed.
 
     Lemma seq_rule c1 c2 P Q R :
       ({{P}}c1{{Q}} //\\ {{Q}}c2{{R}}) |-- {{P}}seq_cmd c1 c2{{R}}.
     Proof.
-      intros n Pr [Hc1 Hc2] Pr' k m s h t HPP' Hmn Hkm HP; split.
-      + intro HFail; inversion HFail; subst; clear HFail.
+      intros Pr n [Hc1 Hc2] Pr' k m s h t HPP' Hmn Hkm HP; split.
+      + intros HFail; inversion HFail; subst; clear HFail.	
         * destruct (Hc1 _ _ n0 s h t HPP' Hmn) as [HS _];
-          [omega | assumption | apply HS; exact H].
+          [omega | assumption | apply HS; assumption ].
         * destruct (Hc1 _ _ n0 s h t HPP' Hmn) as [_ HC]; [omega | assumption |].
           specialize (HC _ _ _ H).
           destruct (Hc2 _ (k - n0) n' s' h' t' HPP') as [HS _]; [omega | omega | |].
-          apply HC. apply HS. exact H0.
-      + intros h1 s1 t1 HSem; inversion HSem; subst; clear HSem.
+          apply HC. 
+          apply HS; exact H0.
+      + intros t' h' s' HSem; inversion HSem; subst; clear HSem.
         destruct (Hc1 _ _  n0 s h t HPP' Hmn) as [_ HC1]; [omega | assumption |].
-        specialize (HC1 _ _ _ H6).
-        destruct (Hc2 _ (k - n0) n1 s2 h2 t2 HPP') as [_ HC2]; [omega | omega | |].
-        apply HC1. specialize (HC2 _ _ _ H8).
-        solve_model HC2.
+        specialize (HC1 _ _ _ H6) (*; destruct HC1 as [HC1 Hst1] *).
+        destruct (Hc2 _ (k - n0) n1 s1 h1 t1 HPP') as [_ HC2]; [omega | omega | |].
+        apply HC1.
+        specialize (HC2 _ _ _ H8) (*; destruct HC2 as [HC2 Hst2] *).
+        (* split. *)
+        * solve_model HC2.
+        (* * intuition. *) 
     Qed.
 
-    Lemma nondet_rule c1 c2 P Q :
+    Lemma nondet_rule c1 c2 P Q:
       ({{P}}c1{{Q}} //\\ {{P}}c2{{Q}}) |-- {{P}}nondet_cmd c1 c2{{Q}}.
     Proof.
       intros n Pr [Hc1 Hc2] Pr' k m s h t HPP' Hmn Hkm HP; split.
-      + intro HFail; inversion HFail; subst; clear HFail.
+      + intros HFail; inversion HFail; subst; clear HFail.
         * destruct (Hc1 _ _ n0 s h t HPP' Hmn) as [HS _];
-          [omega | assumption | apply HS; exact H].
+          [omega | assumption | apply HS; assumption].
         * destruct (Hc2 _ _ n0 s h t HPP' Hmn) as [HS _];
-          [omega | assumption | apply HS; exact H].
+          [omega | assumption | apply HS; assumption].
       + intros h1 s1 t1 HSem; inversion HSem; subst; clear HSem.
         * destruct (Hc1 _ _ n0 s h t HPP' Hmn) as [_ HC]; [omega | assumption |].
-          specialize (HC _ _ _ H5). solve_model HC.
+          specialize (HC _ _ _ H5) (*; destruct HC as [HC Hst] *). 
+          solve_model HC.
+          (* split; [ solve_model HC | assumption ]. *)
         * destruct (Hc2 _ _ n0 s h t HPP' Hmn) as [_ HC]; [omega | assumption |].
-          specialize (HC _ _ _ H5). solve_model HC.
+          specialize (HC _ _ _ H5) (*; destruct HC as [HC Hst] *).
+           solve_model HC.
+          (* split; [ solve_model HC | assumption ]. *)
     Qed.
 
-    Lemma kleene_rule c P :
+    Lemma kleene_rule c P:
       {{P}}c{{P}} |-- {{P}} kleene_cmd c {{P}}.
     Proof.
-      intros n Pr Hc Pr' m k s h t HPP' Hmn Hkm Hp; split.
-      + intro HFail. generalize dependent m. remember None as cfg.
+      intros Pr n Hc Pr' m k s h t HPP' Hmn Hkm Hp; split.
+      + intros HFail. generalize dependent m. remember None as cfg.
         induction HFail; intros; inversion Heqcfg; subst.
         * destruct (Hc _ m n0 s h t HPP' Hmn) as [HS _];
-          [omega | assumption | apply HS; exact H].
+          [omega | assumption | apply HS; assumption].
         * destruct (Hc _ m n0 s h t HPP' Hmn) as [_ HC]; [omega | assumption |].
           apply IHHFail with (m-n0); [assumption | reflexivity | omega | omega | ].
-          specialize (HC _ _ _ H). solve_model HC.
+          specialize (HC _ _ _ H) (*; destruct HC as [HC Hst] *).
+          solve_model HC.
       + intros. remember (Some (s', (h', t'))) as cfg. generalize dependent m. 
         induction H; inversion Heqcfg; subst; intros.
         * solve_model Hp.
+          (* split; [ solve_model Hp | intuition ]. *)
         * destruct (Hc _ m n0 s h t HPP' Hmn) as [_ HC]; [omega | assumption |].
-          assert ((((P s') P0) ((m - n0) - n1)) h') as H1. 
-          apply IHkleene_sem; try assumption; try omega. apply HC in H; assumption.
-          solve_model H1.
+          specialize (HC _ _ _ H) (*; destruct HC as [HC Hst] *).
+          assert ((((P s') t' P0) ((m - n0) - n1)) h') as H2. 
+            apply IHkleene_sem; try assumption; try omega. 
+          (* assert ( (STs_traces P0 (st s') t' -> STs_traces P0 (st s0) t0)).
+            apply IHkleene_sem with (m := m - n0); try assumption; try omega. *)
+          solve_model H2.
+          (* split; [ solve_model H2 | intuition]. *)
     Qed.
 
     Lemma assume_rule P (t : vlogic) :
@@ -174,15 +203,18 @@ Section Rules.
       + intros HFail. inversion HFail.
       + intros tr' h' s' H. remember (Some (s', (h', tr'))) as cfg; induction H.
         inversion Heqcfg; subst; intros.
+        (* split; [| intuition]. *)
         split; [assumption|]. solve_model Hp.
     Qed.
 
     Lemma assert_rule (P : sasn) (p : vlogic) (HPe : P |-- embed p) :
       |-- {{P}} assert_cmd p {{P}}.
     Proof.
-      intros n Pr Hc Pr' m k s h t HPP' Hmn Hkm Hp; specialize (HPe _ _ _ _ Hp); split.
-      + intro HF; inversion HF; subst; auto.
-      + intros t' h' s' HSem; inversion HSem; subst. solve_model Hp.
+      intros n Pr Hc Pr' m k s h t HPP' Hmn Hkm Hp; specialize (HPe _ _ _ _ _ Hp); split.
+      + intros HF; inversion HF; subst; auto.
+      + intros t' h' s' HSem; inversion HSem; subst.
+        solve_model Hp.
+        (* split; [ solve_model Hp | intuition ]. *)
     Qed.
 
   End PrimitivesRules.
@@ -198,7 +230,7 @@ Section Rules.
 
   (* Holds only in one direction unless annotations on assertion logic, which is ugly - well, it's happened. - F.
      This is the important direction, though *)
-  Lemma I_precond (SP : spec) (P Q : sasn) c :
+  Lemma I_precond (SP : spec) (P Q : sasn) c:
     (SP -->> {{ P }} c {{ Q }}) -|- {{ SP /\\  P }} c {{ Q }}.
   Proof.
   	split.
